\documentclass[12pt]{article} 
\usepackage[utf8]{inputenc}
\usepackage{geometry}
\geometry{letterpaper}
\usepackage{graphicx} 
\usepackage{parskip}
\usepackage{booktabs}
\usepackage{array} 
\usepackage{paralist} 
\usepackage{verbatim}
\usepackage{subfig}
\usepackage{fancyhdr}
\usepackage{sectsty}
\usepackage{mathtools}
\usepackage{empheq}
\pagestyle{fancy}
\renewcommand{\headrulewidth}{0pt} 
\lhead{}\chead{}\rhead{}
\lfoot{}\cfoot{\thepage}\rfoot{}

%%% SECTION TITLE APPEARANCE
\allsectionsfont{\sffamily\mdseries\upshape} 

%%% ToC (table of contents) APPEARANCE
\usepackage[nottoc,notlof,notlot]{tocbibind} 
\usepackage[titles,subfigure]{tocloft}
\renewcommand{\cftsecfont}{\rmfamily\mdseries\upshape}
\renewcommand{\cftsecpagefont}{\rmfamily\mdseries\upshape} %

\usepackage{amsmath}
\usepackage{amssymb}

\title{APMA 0350: Homework 10}
\author{Milan Capoor}
\date{2 December 2022}

\begin{document}
\maketitle
\textbf{Problem 1:} Use undetermined coefficients to find the general solution of $x' = Ax + f$ where 
\[A = \begin{bmatrix}
    1 & 1\\
    4 & -2
\end{bmatrix} \quad f = \begin{bmatrix}
    e^{-2t}\\
    -2e^t
\end{bmatrix}\]

Eigenvalues: 
\[\det (A - \lambda I) = 0 \implies (1 - \lambda)(-2 - \lambda) - 4 = 0\]
\[\lambda^2 + \lambda - 6 = (\lambda + 3)(\lambda - 2) = 0\]
\[\lambda = \{2, \; -3\}\]

Eigenvector $\lambda = 2$:
\[\left[\begin{array}{c c | c}
    -1 & 1 & 0\\
    4 & -4 & 0
\end{array}\right] \implies -x_1 + x_2 = 0\]
\[\vec{v}_{\lambda = 2} = \begin{bmatrix}
    1\\1
\end{bmatrix}\]

Eigenvector $\lambda = -3$:
\[\left[\begin{array}{c c | c}
    4 & 1 & 0\\
    4 & 1 & 0
\end{array}\right] \implies 4x_1 + x_2 = 0\]
\[\vec{v}_{\lambda = -3} = \begin{bmatrix}
    1\\-4
\end{bmatrix}\]

Homogeneous solution:
\[x_0 = Ae^{2t} \begin{bmatrix}
    1\\1
\end{bmatrix} + Be^{-3t} \begin{bmatrix}
    1\\-4
\end{bmatrix}\]

Roots of inhomogeneous term: $r = \{-2, \; 1\} \longrightarrow$ (no resonance)

Particular solution:
\[f = e^{-2t} \begin{bmatrix}
    1\\0
\end{bmatrix} + e^t \begin{bmatrix}
    0\\-2
\end{bmatrix}\]
\[x_p = e^{-2t} \begin{bmatrix}
    A\\B
\end{bmatrix} + e^t \begin{bmatrix}
    C\\D\
\end{bmatrix} = \begin{bmatrix}
    Ae^{-2t} + Ce^t\\
    Be^{-2t} + De^t
\end{bmatrix}\]

\[x_p' = Ax_p + f\]
\begin{align*}
    \begin{bmatrix}
        -2Ae^{2t} + Ce^t\\
        -2Be^{-2t} + De^t
    \end{bmatrix} &= \begin{bmatrix}
    1 & 1\\
    4 & -2
    \end{bmatrix} \begin{bmatrix}
        Ae^{-2t} + Ce^t\\
        Be^{-2t} + De^t
    \end{bmatrix} + \begin{bmatrix}
        e^{-2t}\\
        -2e^t
    \end{bmatrix}\\
    &= \begin{bmatrix}
        Ae^{-2t} + Be^{-2t} + Ce^t + De^t\\
        4Ae^{-2t} + 4Ce^t - 2Be^{-2t} - 2De^t
    \end{bmatrix} + \begin{bmatrix}
        e^{-2t}\\
        -2e^t
    \end{bmatrix}\\
    &= \begin{bmatrix}
        Ae^{-2t} + Be^{-2t} + Ce^t + De^t + e^{-2t}\\
        4Ae^{-2t} + 4Ce^t - 2Be^{-2t} - 2De^t -2e^t
    \end{bmatrix}\\
    &= \begin{bmatrix}
        (A + B + 1)e^{-2t} + (C + D)e^t\\
        (4A - 2B)e^{-2t} + (4C - 2D - 2)e^t
    \end{bmatrix}
\end{align*}

\[\begin{cases}
    A + B + 1 = -2A\\
    C + D = C\\
    4A - 2B = -2B\\
    4C - 2D - 2 = D
\end{cases} \implies \begin{cases}
    A = 0\\
    B = -1\\
    C = 1/2\\
    D = 0
\end{cases}\]

\[x_p = \begin{bmatrix}
    Ae^{-2t} + Ce^t\\
    Be^{-2t} + De^t
\end{bmatrix}\]

\[x_p = \begin{bmatrix}
    \frac{1}{2}e^t\\
    -e^{-2t}
\end{bmatrix}\]

General solution:
\[x = x_0 + x_p\]
\[x = Ae^{2t} \begin{bmatrix}
    1\\1
\end{bmatrix} + Be^{-3t} \begin{bmatrix}
    1\\-4
\end{bmatrix} + \begin{bmatrix}
    \frac{1}{2}e^t\\
    -e^{-2t}
\end{bmatrix}\]
\[\boxed{x = \begin{bmatrix}
    Ae^{2t} + Be^{-3t} + \frac{1}{2}e^t\\
    Ae^{2t} - 4Be^{3t} - e^{-2t}
\end{bmatrix}}\]

\pagebreak

\textbf{Problem 2:} Guess the form of a particular
solution to $x' = Ax + f$ where
\[A = \begin{bmatrix}
    2 & -1\\
    -1 & 2
\end{bmatrix}\]
\[\det (A - \lambda I) = (2 - \lambda)^2 - 1 = \lambda^2 - 4\lambda + 3 = (\lambda - 3)(\lambda - 1)\]
\[\lambda = \{1, \; 3\}\]

\begin{enumerate}
    \item \[\mathbf{f = \begin{bmatrix}
        e^{2t}\\
        2e^{2t}
    \end{bmatrix}}\]

    Solution:
    \[f = e^{2t} \begin{bmatrix}
        1\\2
    \end{bmatrix} \quad (\lambda = 2)\]
    No resonance so 
    \[\boxed{x_p = \begin{bmatrix}
        Ae^{2t}\\
        Be^{2t}
    \end{bmatrix}}\]

    \item \[\mathbf{f = \begin{bmatrix}
        3e^{2t}\\
        -e^{4t}
    \end{bmatrix}}\]

    Solution:
    \[f = e^{2t} \begin{bmatrix}
        3\\0
    \end{bmatrix} + e^{4t} \begin{bmatrix}
        0\\-1
    \end{bmatrix} \quad (\lambda = \{2, \; 4\})\]
    No resonance so 
    \[\boxed{x_p = e^{2t} \begin{bmatrix}
        A\\B
    \end{bmatrix} + e^{4t} \begin{bmatrix}
        C\\D
    \end{bmatrix}}\]

    \item \[\mathbf{f = \begin{bmatrix}
        \cos (2t)\\
        \sin (3t)
    \end{bmatrix}}\]

    Solution: 
    \[\boxed{x_p = \cos(2t) \begin{bmatrix}
        A\\B
    \end{bmatrix} + \sin(2t) \begin{bmatrix}
        C\\D
    \end{bmatrix} + \cos(3t) \begin{bmatrix}
        E\\F
    \end{bmatrix} + \sin(3t) \begin{bmatrix}
        G\\H
    \end{bmatrix}}\]
   
    \item \[\mathbf{f = \begin{bmatrix}
        t^2\\
        te^{5t}
    \end{bmatrix}}\]

    Solution:
    \[\begin{bmatrix}
        At^2 + Ct\\
        bt^2 + Dt
    \end{bmatrix}e^{5t}\]
\end{enumerate}

\pagebreak 

\textbf{Problem 3:} Use variation of parameters to find the general solution of the following ODE. Simplify your answers.
\begin{enumerate}
    \item \[\mathbf{y'' + 4y' + 4y = \frac{e^{-2t}}{t^2}}\]
    Homogeneous equation: 
    \[r^2 + 4r + 4 = (r + 2)^2 = 0 \implies r = -2 \quad (\text{repeated})\]
    \[y_0 = Ae^{-2t} + Bte^{-2t}\]

    Var par equations:
    \[\begin{bmatrix}
        e^{-2t} & te^{-2t}\\
        -2e^{-2t} & e^{-2t} -2te^{-2t}
    \end{bmatrix} \begin{bmatrix}
        u'\\
        v'
    \end{bmatrix} = \begin{bmatrix}
        0\\
        \frac{e^{-2t}}{t^2}
    \end{bmatrix}\] 

    \[u'(t) = \frac{\begin{vmatrix}
       0 & te^{-2t}\\
       \frac{e^{-2t}}{t^2} & e^{-2t} -2te^{-2t}
    \end{vmatrix}}{\begin{vmatrix}
        e^{-2t} & te^{-2t}\\
        -2e^{-2t} & e^{-2t} -2te^{-2t}
    \end{vmatrix}} = \frac{-\frac{e^{-4t}}{t}}{e^{-4t} -2te^{-4t} + 2te^{-4t}}\]
    \[= \frac{-e^{-4t}}{te^{-4t} -2t^2e^{-4t} + 2t^2e^{-4t}} = \frac{1}{t}\]

    \[v'(t) = \frac{\begin{vmatrix}
        e^{-2t} & 0\\
         -2e^{-2t} & \frac{e^{-2t}}{t^2} 
     \end{vmatrix}}{\begin{vmatrix}
         e^{-2t} & te^{-2t}\\
         -2e^{-2t} & e^{-2t} -2te^{-2t} \end{vmatrix}} 
    = \frac{\frac{e^{-4t} }{t^2}}{e^{-4t} -2te^{-4t} + 2te^{-4t}} = \frac{1}{t^2}\]      
         
    \[\begin{cases}
        u'(t) = -\frac{1}{t}\\
        v'(t) = \frac{1}{t^2}
    \end{cases} \implies \begin{cases}
        u(t) = -\ln |t|\\
        v(t) = -\frac{1}{t}
    \end{cases}\]

    Particular solution: 
    \[y_p(t) = u(t) e^{-2t} + v(t) t e^{-2t}\]
    \[y_p(t) = -\ln |t| e^{-2t} - e^{-2t}\]

    General solution:
    \[\boxed{y = Ae^{-2t} + Bte^{-2t} - \ln |t| e^{-2t} - e^{-2t}}\]


    \item \[\mathbf{t^2 y'' - t(t+2)y' + (t+2)y = 2t^3}\]
\end{enumerate}

\pagebreak 

\textbf{Problem 4:} Use variation of parameters to find the general solution of $x' = Ax + f$ where
\[\mathbf{A = \begin{bmatrix}
    2 & -1\\
    3 & -2
\end{bmatrix} \quad f = e^t \begin{bmatrix}
    1\\
    -1
\end{bmatrix}}\]

Homogeneous solution:
\[\det (A - \lambda I) = (2 - \lambda)(-2 - \lambda) + 3 = \lambda^2 - 1 = (\lambda + 1)(\lambda - 1) = 0\]
\[\lambda = \{-1, \; 1\}\]

Eigenvector $\lambda = -1$:
\[\left[\begin{array}{c c | c}
    3 & -1 & 0\\
    3 & -1 & 0
\end{array}\right] \implies 3x_1 - x_2 =0 \]
\[\vec{v}_{\lambda = -1} = \begin{bmatrix}
    1\\3
\end{bmatrix}\]

Eigenvector $\lambda = 1$:
\[\left[\begin{array}{c c | c}
    1 & -1 & 0\\
    3 & -3 & 0
\end{array}\right] \implies x_1 - x_2 = 0\]
\[\vec{v}_{\lambda = 1} = \begin{bmatrix}
    1\\1
\end{bmatrix}\]

\[x_0 = Ae^{-t}\begin{bmatrix}
    1\\3
\end{bmatrix} + Be^t \begin{bmatrix}
    1\\1
\end{bmatrix} = A\begin{bmatrix}
    e^{-t}\\
    3e^{-t}
\end{bmatrix} + B \begin{bmatrix}
    e^t\\
    e^t
\end{bmatrix}\]

Particular solution:
\[x_p = u(t)\begin{bmatrix}
    e^{-t}\\
    3e^{-t}
\end{bmatrix} + v(t) \begin{bmatrix}
    e^t\\
    e^t
\end{bmatrix}\]

\[\begin{bmatrix}
    e^{-t} & e^t\\
    3e^{-t} & e^t
\end{bmatrix} \begin{bmatrix}
    u'\\
    v'
\end{bmatrix} = \begin{bmatrix}
    e^t\\
    e^{-t}
\end{bmatrix}\]

\[u' = \frac{\begin{vmatrix}
    e^{t} & e^t\\
    e^{-t} & e^t
\end{vmatrix}}{\begin{vmatrix}
    e^{-t} & e^t\\
    3e^{-t} & e^t
\end{vmatrix}} = \frac{e^{2t} - 1}{-2} = \frac{-e^{2t}}{2} + \frac{1}{2}\]

\[v' = \frac{\begin{vmatrix}
    e^{-t} & e^t\\
    3e^{-t} & e^{-t}
\end{vmatrix}}{\begin{vmatrix}
    e^{-t} & e^t\\
    3e^{-t} & e^t
\end{vmatrix}} = \frac{e^{-2t} - 3}{-2} = \frac{-e^{2t}}{2} + \frac{3}{2}\]
\[\begin{cases}
    u'(t) = \frac{-e^{2t}}{2} + \frac{1}{2}\\
    v'(t) = \frac{-e^{2t}}{2} + \frac{3}{2}
\end{cases} \implies \begin{cases}
    u = \int \frac{-e^{2t}}{2} + \frac{1}{2}\; dt = \frac{-e^{2t}}{4} + \frac{t}{2}\\
    v= \int \frac{-e^{2t}}{2} + \frac{4}{2}\; dt = \frac{-e^{2t}}{4} + \frac{3t}{2}\\
\end{cases}\]

\[x_p = \left(\frac{-e^{2t}}{4} + \frac{t}{2}\right)\begin{bmatrix}
    e^{-t}\\
    3e^{-t}
\end{bmatrix} + \left(\frac{-e^{2t}}{4} + \frac{3t}{2}\right) \begin{bmatrix}
    e^t\\
    e^t
\end{bmatrix}\]

\[x_p = \begin{bmatrix}
    -\frac{1}{4}e^t + \frac{1}{2}te^{-t}\\
    -\frac{3}{4}e^t + \frac{3}{2}te^{-t}
\end{bmatrix} + \begin{bmatrix}
    -\frac{1}{4}e^t + \frac{3}{2}te^{-t}\\
    -\frac{3}{4}e^t + \frac{9}{2}te^{-t}
\end{bmatrix} = \begin{bmatrix}
    -\frac{1}{2}e^t + 2te^{-t}\\
    -\frac{3}{2}e^t + 6te^{-t}
\end{bmatrix}\]

General solution:
\[\boxed{x = A\begin{bmatrix}
    e^{-t}\\
    3e^{-t}
\end{bmatrix} + B \begin{bmatrix}
    e^t\\
    e^t
\end{bmatrix} + \begin{bmatrix}
    -\frac{1}{2}e^t + 2te^{-t}\\
    -\frac{3}{2}e^t + 6te^{-t}
\end{bmatrix}}\]

\pagebreak

\textbf{Problem 5:} Find the general solution of $y'' + y = cos(t)$
\begin{enumerate}
    \item Using undetermined coefficients
    \[r^2 + r = 0 \implies r(r + 1) = 0 \implies r = \{0, \; 1\}\]
    \[\cos t \implies r = 1\]
    So we have resonance! 
    \[y_0 = A + Bte^{t}\]

    \[x_p = A\cos(t) + B\sin(t)\]
    \[(A\cos(t) + B\sin(t))'' + (A\cos(t) + B\sin(t)) = \cos t\]
    \[-A\cos(t) - B\sin t + A \cos t + B \sin t\]
    \[\cos t = 0\]
    
    \item Using variation of parameters
    \[r^2 + r = 0 \implies r(r + 1) = 0 \implies r = \{0, \; 1\}\]
    \[y_0 = A + Be^t\]
    \[y_p = u(t) + v(t) e^t\]
    \[\begin{bmatrix}
        1 & e^t\\
        0 & e^t
    \end{bmatrix} \begin{bmatrix}
        u'\\
        v'
    \end{bmatrix} = \begin{bmatrix}
        0\\
        cos(t)
    \end{bmatrix}\]

    \[u' = \frac{\begin{vmatrix}
        0 & e^t\\
        \cos t & e^t
    \end{vmatrix}}{\begin{vmatrix}
        1 & e^t\\
        0 & e^t
    \end{vmatrix}} = \frac{-e^t\cos t}{e^t} = - \cos t \implies u = - \sin t\]

    \[v' = \frac{\begin{vmatrix}
        1 & 0\\
        0 & \cos t
    \end{vmatrix}}{\begin{vmatrix}
        1 & e^t\\
        0 & e^t
    \end{vmatrix}} = \frac{-\cos t}{e^t} \implies v = \frac{1}{2}e^{-t}\left(\cos t - \sin t\right) \]
    
    \[y_p = -\sin t + \frac{1}{2} \cos t - \frac{1}{2} \sin t = -\frac{3}{2}\sin t + \frac{1}{2} \cos t\]

    General solution:
    \[\boxed{y = A + Be^t -\frac{3}{2}\sin t + \frac{1}{2} \cos t }\]
\end{enumerate}
\end{document}